parallelism

PSBP/Implementations/ProgramImplementations.lean
@@ -2,30 +2,31 @@ import PSBP.Specifications.ProgramSpecifications
 
 import PSBP.Structures.ComputationValuedFunction
 
+import PSBP.Implementations.ReactiveImplementations
+
 instance [Applicative computation] :
     Functional
       (FromComputationValuedFunction computation) where
   asProgram :=
-    λ αfβ => ⟨λ α => pure $ αfβ α⟩
+    λ αfβ ↦ ⟨λ α ↦ pure $ αfβ α⟩
 
 instance [Functor computation] :
     Functorial
       (FromComputationValuedFunction computation) where
   andThenF :=
-    λ ⟨αfcβ⟩ βfγ => ⟨λ α => βfγ <$> αfcβ α⟩
+    λ ⟨αfcβ⟩ βfγ ↦ ⟨λ α ↦ βfγ <$> αfcβ α⟩
 
 instance [Monad computation] :
     Sequential
       (FromComputationValuedFunction computation) where
-  andThen :=
-    λ ⟨αfcβ⟩ ⟨βfcγ⟩ => ⟨λ α => αfcβ α >>= βfcγ⟩
+  andThenP :=
+    λ ⟨αfcβ⟩ ⟨βfcγ⟩ ↦ ⟨λ α ↦ αfcβ α >>= βfcγ⟩
 
 instance [Applicative computation] :
     Creational
       (FromComputationValuedFunction computation) where
-  product := λ ⟨αfcβ⟩ ⟨αfcγ⟩ =>
-    -- ⟨λ α => pure .mk <*> αfcβ α <*> αfcγ α⟩
-    ⟨λ α => .mk <$> αfcβ α <*> αfcγ α⟩
+  productSeq := λ ⟨αfcβ⟩ ⟨αfcγ⟩ ↦
+    ⟨λ α ↦ .mk <$> αfcβ α <*> αfcγ α⟩
 
 def foldSum {γ β α : Type}
     (γfα : γ → α)
@@ -38,4 +39,27 @@ def foldSum {γ β α : Type}
 instance :
     Conditional
       (FromComputationValuedFunction computation) where
-  sum := λ ⟨γfγα⟩ ⟨βfγα⟩ => ⟨foldSum γfγα βfγα⟩
+  sum := λ ⟨γfγα⟩ ⟨βfγα⟩ ↦ ⟨foldSum γfγα βfγα⟩
+
+instance : Monad Task where
+  pure := Task.pure
+  bind := Task.bind
+
+class MonadAsync
+    (computation : Type → Type) where
+  async {α : Type} (ufα : Unit → α) : computation α
+
+export MonadAsync (async)
+
+instance : MonadAsync Task where
+  async := Task.spawn
+
+instance
+    [Monad computation]
+    [MonadAsync computation] :
+  Parallel (FromComputationValuedFunction computation) where
+    bothPar := λ ⟨αfcγ⟩ ⟨βfcδ⟩ =>
+      ⟨λ ⟨α, β⟩ =>
+        async (λ (_: Unit) => αfcγ α) >>=
+          λ cγ => async (λ (_: Unit) => βfcδ β) >>=
+            λ cδ => .mk <$> cγ <*> cδ⟩
