PSBP/Structures/ComputationValuedFunction.lean
@@ -1,3 +1,3 @@
 structure FromComputationValuedFunction
-    (computation : (Type → Type)) (α β : Type) where
+    (computation : Type → Type) (α β : Type) where
   toComputationValuedFunction : α → computation β
