PSBP/Implementations/GenericImplementations.lean
@@ -5,10 +5,10 @@ import PSBP.Specifications.PositionalSpecification
 instance
     [Functional program]
     [Sequential program] :
-    Functorial program where
-  andThenF {α β γ: Type} :
-    program α β → (β → γ) → program α γ :=
-      λ αpβ βfγ => αpβ >=> asProgram βfγ
+  Functorial program where
+    andThenF {α β γ: Type} :
+      program α β → (β → γ) → program α γ :=
+        λ αpβ βfγ => αpβ >=> asProgram βfγ
 
 instance
     [Functional program]
