PSBP/Laws/WithStateLaws.lean
@@ -1,0 +1,30 @@
+import PSBP.Specifications.ProgramSpecifications
+
+import PSBP.Specifications.WithStateSpecification
+
+import PSBP.Structures.ComputationValuedFunction
+
+class LawfulStateOf (computation : Type → Type)
+    [Monad computation]
+    [MonadStateOf σ computation] : Prop where
+  stateOf_write_read :
+    (λ σ => set σ >>= λ _ : PUnit => get) =
+      (pure : σ → computation σ)
+
+@[simp] theorem stateOf_write_read_theorem
+  {σ : Type}
+    [Monad computation]
+    [MonadStateOf σ computation] :
+  (λ σ => set σ >>= λ _ : PUnit => get
+    : σ → computation σ ) =
+      (pure : σ → computation σ) :=
+        sorry
+
+class LawfulWithState (program : Type → Type → Type)
+    [Functional program]
+    [Sequential program]
+    [WithState σ program] : Prop where
+  withState_write_read :
+    (writeState >=> (readState : program Unit σ)) =
+      identity
+
