PSBP/Materializations/ActiveMaterialization.lean
@@ -2,9 +2,9 @@ import PSBP.Structures.ComputationValuedFunction
 
 import PSBP.Implementations.ActiveImplementations
 
-abbrev ActiveProgram α β :=
-  FromComputationValuedFunction Active α β
+abbrev ActiveProgram :=
+  FromComputationValuedFunction Active
 
 def materializeActive :
     ActiveProgram α β → (α → β) :=
-  λ ⟨αfaβ⟩ α => (αfaβ α).run
+  λ ⟨αfaβ⟩ α => αfaβ α -- .run
