PSBP/Materializations/TaskMaterialization.lean
@@ -1,0 +1,11 @@
+import PSBP.Structures.ComputationValuedFunction
+
+import PSBP.Implementations.ProgramImplementations
+
+abbrev TaskProgram :=
+  FromComputationValuedFunction Task
+
+def materializeTask {α β : Type} :
+  TaskProgram α β → (α → β) :=
+    λ ⟨αftβ⟩ α => (αftβ α).get
+
