PSBP/Programs/Programs.lean
@@ -4,8 +4,8 @@ import PSBP.Programs.PrimitivePrograms
 
 unsafe def fibonacci
     [Functional program]
-    [Creational program]
     [Sequential program]
+    [Creational program]
     [Conditional program] :
   program Nat Nat :=
     if_ isZero one $
@@ -16,8 +16,23 @@ unsafe def fibonacci
             (minusTwo >=> fibonacci) >=>
             add
 
+-- exercise
+unsafe def fibonacci'
+    [Functional program]
+    [Sequential program]
+    [Creational program]
+    [Sequential program]
+    [Conditional program] :
+  program Nat Nat :=
+    if_ isZero one $
+      if_ isOne one $
+        (minusOne >=> fibonacci') &&&
+        (minusTwo >=> fibonacci') >=>
+        add
+
 unsafe def factorial
     [Functional program]
+    [Sequential program]
     [Creational program]
     [Sequential program]
     [Conditional program] :
@@ -28,14 +43,54 @@ unsafe def factorial
           in_ $
             multiply
 
-def twiceMinusOne01
+-- exercise
+unsafe def factorial'
+    [Functional program]
+    [Sequential program]
+    [Creational program]
+    [Sequential program]
+    [Conditional program] :
+  program Nat Nat :=
+    if_ isZero one $
+      let_ (minusOne >=> factorial') $
+        multiply
+
+unsafe def fibonacci''
+    [Functional program]
+    [Sequential program]
+    [Creational program]
+    [Conditional program] :
+  program Nat Nat :=
+    if_ isZero one $
+      else_ $
+        if_ isOne one $
+          else_ $
+            (dup >=>
+            (minusOne >=> fibonacci') <&>
+            (minusTwo >=> fibonacci')) >=>
+            add
+
+unsafe def parallelFibonacci
+    [Functional program]
+    [Sequential program]
+    [Creational program]
+    [Conditional program]
+    [Parallel program] :
+  program Nat Nat :=
+    if_ isZero one $
+      if_ isOne one $
+        (minusOne >=> parallelFibonacci) &|&
+        (minusTwo >=> parallelFibonacci) >=>
+        add
+
+def twiceMinusOneFunctorial
     [Functional program]
     [Functorial program]
     [Creational program] :
   program Nat Nat :=
     minusOne &&& minusOne >-> addF
 
-def twiceMinusOne02
+def twiceMinusOneSequential
     [Functional program]
     [Sequential program]
     [Creational program] :
