PSBP/Theorems/WithStateTheorems.lean
@@ -1,0 +1,3 @@
+def foo : Nat := 1
+
+
